Add eval rules for STLC

proof/Main.v
@@ -1,30 +1,33 @@
 
 Require Import Base.
 Require Import Name.
+Require Import Exp.
+Require Import Ty.
 
- 
+(* evaluation *********************************************)
+Inductive STEP : exp -> exp -> Prop := 
+  | EVAppAbs 
+    :   forall x T t12 v2 
+    ,   VALUE v2 
+    ->  STEP  (XApp (XLam x T t12) v2)
+              (subst x v2 t12)
 
-(* types **************************************************)
-Inductive ty : Type :=
- | TVar  : name -> ty
- | TFun  : ty -> ty -> ty.
+  | EVApp1 
+    :   forall t1 t1' t2
+    ,   STEP t1 t1'
+    ->  STEP (XApp t1 t2) (XApp t1' t2)
 
-Notation A := (TVar (Name 0)).
-Notation B := (TVar (Name 1)).
-Notation C := (TVar (Name 2)).
-
-
-(* terms **************************************************)
-Inductive exp : Type :=
- | XVar  : name -> exp
- | XApp  : exp  -> exp -> exp
- | XLam  : name -> ty  -> exp -> exp.
-
-
-
+  | EVApp2
+    :   forall v1 t2 t2'
+    ,   VALUE v1
+    ->  STEP  t2 t2'
+    ->  STEP  (XApp v1 t2) (XApp v1 t2').
 
 
+Example xIdA := XLam nA tA (XVar nA).
 
+Lemma example_step1 : STEP (XApp xIdA (XAtom nB)) (XAtom nB).
+Proof. unfold xIdA. apply EVAppAbs. auto. Qed.
 
 
 
