proof/Exp.v
@@ -1,0 +1,49 @@
+
+Require Export Name.
+Require Export Ty.
+Require Export Cases.
+
+(* expressions *******************************************)
+Inductive exp : Type :=
+  | XAtom : name -> exp
+  | XVar  : name -> exp
+  | XLam  : name -> ty  -> exp -> exp
+  | XApp  : exp  -> exp -> exp.
+
+
+Tactic Notation "exp_cases" tactic(first) ident(c) :=
+  first;
+  [ Case_aux c "XAtom"
+  | Case_aux c "XVar" 
+  | Case_aux c "XLam"
+  | Case_aux c "XApp" ]. 
+
+
+(* values **************************************************)
+Inductive VALUE : exp -> Prop :=
+ | VALUE_XAtom : forall x,     VALUE (XAtom x)
+ | VALUE_XLam  : forall x T t, VALUE (XLam x T t).
+
+Hint Constructors VALUE.
+
+
+(* substitution *******************************************)
+(* TODO: only works for s closed *)
+
+Fixpoint subst (n : name) (s : exp) (t : exp) : exp :=
+  match t with
+    |  XAtom _
+    => t
+
+    |  XVar n'      
+    => if beq_name n n' then s else t
+
+    |  XLam n' T x1
+    => XLam n' T 
+         (if beq_name n n'
+              then x1
+              else subst n s x1)
+
+    |  XApp x1 x2 
+    => XApp (subst n s x1) (subst n s x2)
+  end.
